Breaking up into files

LambdaO.v
@@ -9,10 +9,8 @@ Require Import Bedrock.Platform.Cito.ListFacts4.
 Require Import Bedrock.Platform.Cito.GeneralTactics.
 Require Import Bedrock.Platform.Cito.GeneralTactics3.
 Require Import NonnegRational.
-Require Import Syntax.
 Require Import Util.
-Require Import Subst.
-Require Import Order.
+Require Import TypingFacts.
 
 Import ListNotations.
 Open Scope list_scope.
@@ -51,298 +49,17 @@ Instance Functor_assoc_list A : Functor (assoc_list A) :=
     map := @map_assoc_list A
   }.
 
-Infix "<<" := compose (at level 40) : prog_scope.
-Infix ">>" := (flip compose) (at level 40) : prog_scope.
-Open Scope prog_scope.
-
-Instance Apply_type_type_type : Apply type type type :=
-  {
-    apply := Tapp
-  }.
-
-Definition Tunit := Tconstr TCunit.
-Definition Tprod t1 t2 := Tconstr TCprod $$ t1 $$ t2.
-Definition Tsum t1 t2 := Tconstr TCsum $$ t1 $$ t2.
-
-Class Find key value container := 
-  {
-    find : key -> container -> option value
-  }.
-
-Instance Find_list A : Find nat A (list A) :=
-  {
-    find k c := @nth_error A c k
-  }.
-
-Instance Apply_expr_expr_expr : Apply expr expr expr :=
-  {
-    apply := Eapp
-  }.
-
-Instance Apply_expr_type_expr : Apply expr type expr :=
-  {
-    apply := Etapp
-  }.
-
-Definition Epair := Econstr Cpair.
-Definition Einl := Econstr Cinl.
-Definition Einr := Econstr Cinr.
-Definition Ett := Econstr Ctt.
-
-(* kinds are restricted to the form (* => * => ... => *). 0 means * *)
-Definition kind := nat.
-
-(* Typing context.
-   The second field of TEtyping is the optional size constraint
- *)
-Inductive tc_entry := 
-  | TEtyping (_ : type * option size)
-  | TEkinding (_ : kind).
-
 Arguments rev {A} _.
 
 Definition cat_options {A} (ls : list (option A)) := fold_right (fun x acc => match x with Some v => v :: acc | _ => acc end) [] ls.
 
 Definition map_option {A B} (f : A -> option B) := cat_options << map f.
 
-(* Definition tcontext := StringMap.t tc_entry. *)
-Definition tcontext := list tc_entry.
-
 Fixpoint repeat A (a : A) n :=
   match n with
     | O => nil
     | S n => a :: repeat a n
   end.
-
-Arguments fst {A B} _.
-
-Instance Shift_option `{Shift A} : Shift (option A) :=
-  {
-    shift_from n o := option_map (shift_from n) o
-  }.
-
-Instance Shift_pair `{Shift A, Shift B} : Shift (A * B) :=
-  {
-    shift_from n p := (shift_from n (fst p), shift_from n (snd p))
-  }.
-
-Definition add_typing t T := TEtyping t :: T.
-Definition add_typings ls T := fst $ fold_left (fun (p : tcontext * nat) t => let (T, n) := p in (add_typing (shiftby n t) T, S n)) ls (T, 0%nat).
-Definition add_kinding k T := TEkinding k :: T.
-
-Coercion var_to_size (x : var) : size := Svar (x, []).
-
-Inductive kinding : tcontext -> type -> kind -> Prop :=
-| Kvar T n k : find n T = Some (TEkinding k) -> kinding T #n k
-| Kapp T t1 t2 k :
-    kinding T t1 (S k) ->
-    kinding T t2 0 ->
-    kinding T (Tapp t1 t2) k
-| Kabs T t k :
-    kinding (add_kinding 0 T) t k ->
-    kinding T (Tabs t) (S k)
-| Karrow T t1 f g t2 :
-    kinding T t1 0 ->
-    kinding (add_typing (t1, None) T) t2 0 ->
-    kinding T (Tarrow t1 f g t2) 0
-| Kuniversal T f g t :
-    kinding (add_kinding 0 T) t 0 ->
-    kinding T (Tuniversal f g t) 0
-| Krecur T t :
-    kinding (add_kinding 0 T) t 0 ->
-    kinding T (Trecur t) 0
-| Khide T t :
-    kinding T t 0 ->
-    kinding T (Thide t) 0
-| Kunit T :
-    kinding T (Tconstr TCunit) 0
-| Kprod T :
-    kinding T (Tconstr TCprod) 2
-| Ksum T :
-    kinding T (Tconstr TCsum) 2
-(* | Kint T : *)
-(*     kinding T (Tconstr TCint) 0 *)
-.
-
-Inductive teq : type -> type -> Prop :=
-| Qrefl t : teq t t
-| Qsymm a b : teq a b -> teq b a
-| Qtrans a b c : teq a b -> teq b c -> teq a c
-| Qabs a b :
-    teq a b ->
-    teq (Tabs a) (Tabs b)
-| Qapp a b a' b' :
-    teq a a' ->
-    teq b b' ->
-    teq (Tapp a b) (Tapp a' b')
-| Qbeta t1 t2 :
-    teq (Tapp (Tabs t1) t2) (subst t2 t1)
-| Qarrow a f g b a' b' : 
-    teq a a' ->
-    teq b b' ->
-    teq (Tarrow a f g b) (Tarrow a' f g b')
-| Qrecur a b :
-    teq a b ->
-    teq (Trecur a) (Trecur b)
-.
-
-Global Add Relation type teq
-    reflexivity proved by Qrefl
-    symmetry proved by Qsymm
-    transitivity proved by Qtrans
-      as teq_rel.
-
-Class Equal t :=
-  {
-    equal : t -> t -> Prop
-  }.
-
-Infix "==" := equal (at level 70) : G.
-
-Instance Equal_type : Equal type :=
-  {
-    equal := teq
-  }.
-
-Definition add_snd {A B} (b : B) (a : A) := (a, b).
-
-Close Scope F01.
-Open Scope F.
-Open Scope G.
-
-Notation Tuniversal0 := (Tuniversal F0 Stt).
-
-Inductive typing : tcontext -> expr -> type -> cexpr -> size -> Prop :=
-| TPvar T n t s : 
-    find n T = Some (TEtyping (t, s)) -> 
-    typing T #n (shiftby (S n) t) F0 (default (var_to_size #n) (shiftby (S n) s))
-| TPapp T e1 e2 ta tb n s n1 n2 nouse s2 : 
-    typing T e1 (Tarrow ta n s tb) n1 nouse ->
-    typing T e2 ta n2 s2 ->
-    typing T (Eapp e1 e2) (subst s2 tb) (n1 + n2 + F1 + subst s2 n) (subst s2 s)
-| TPabs T e t1 t2 n s :
-    kinding T t1 0 ->
-    typing (add_typing (t1, None) T) e t2 n s ->
-    typing T (Eabs t1 e) (Tarrow t1 n s t2) F0 Stt
-| TPtapp T e t2 n s t n' :
-    typing T e (Tuniversal (shift n) (shift s) t) n' Stt ->
-    typing T (Etapp e t2) (subst t2 t) (n' + F1 + n) s
-| TPtabs T e n s t :
-    typing (add_kinding 0 T) e t n s ->
-    typing T (Etabs e) (Tuniversal n s t) F0 Stt
-| TPlet T t1 e1 e2 t2 n1 n2 s1 s2:
-    typing T e1 t1 n1 s1 ->
-    typing (add_typing (t1, Some s1) T) e2 t2 n2 s2 ->
-    typing T (Elet t1 e1 e2) (subst s1 t2) (n1 + subst s1 n2) (subst s1 s2)
-| TPletrec T (defs : list letrec_entry) main t n s :
-    let len := length defs in
-    let T' := add_typings (map (fst >> fst >> add_snd (Some Stt)) defs) T in
-    (forall lhs_t rhs_t e, 
-       In (lhs_t, rhs_t, e) defs -> 
-       typing T' (Eabs rhs_t e) (shiftby len lhs_t) F0 Stt) ->
-    typing T' main (shiftby len t) (shiftby len n) (shiftby len s) ->
-    typing T (Eletrec defs main) t n s
-| TPmatch_pair T e e' t t1 t2 n s n' s' s1 s2 :
-    typing T e (Tprod t1 t2) n s ->
-    is_pair s = Some (s1, s2) ->
-    let t12 := [(t1, Some s1); (t2, Some s2)] in
-    let T' := add_typings t12 T in
-    typing T' e' t n' s' ->
-    let s12 := [s1; s2] in
-    typing T (Ematch_pair e e') (subst_list s12 t) (n + F1 + subst_list s12 n') (subst_list s12 s')
-| TPmatch_inlinr T e e1 e2 t1 t2 n s s1 s2 t n1 n2 s' :
-    typing T e (Tsum t1 t2) n s ->
-    is_inlinr s = Some (s1, s2) ->
-    (* timing constraints are passed forward; size and type constraints are passed backward.
-       t' and s' are backward guidance for branches *)
-    typing (add_typing (t1, Some s1) T) e1 (shift t) n1 (shift s') -> 
-    typing (add_typing (t2, Some s2) T) e2 (shift t) n2 (shift s') -> 
-    typing T (Ematch_sum e e1 e2) t (n + F1 + max (subst s1 n1) (subst s2 n2)) s'
-| TPmatch_inl T e e1 e2 t1 t2 n s t' n' s' :
-    typing T e (Tsum t1 t2) n (Sinl s) ->
-    typing (add_typing (t1, Some s) T) e1 t' n' s' ->
-    typing T (Ematch_sum e e1 e2) (subst s t') (n + F1 + subst s n') (subst s s')
-| TPmatch_inr T e e1 e2 t1 t2 n s t' n' s' :
-    typing T e (Tsum t1 t2) n (Sinr s) ->
-    typing (add_typing (t2, Some s) T) e2 t' n' s' ->
-    typing T (Ematch_sum e e1 e2) (subst s t') (n + F1 + subst s n') (subst s s')
-| TPfold T e t n s t1 :
-    t == Trecur t1 ->
-    typing T e (subst t t1) n s ->
-    typing T (Efold t e) t n (Sfold s)
-| TPunfold T e t n s s1 t1 :
-    typing T e t n s ->
-    is_fold s = Some s1 ->
-    t == Trecur t1 ->
-    typing T (Eunfold t e) (subst t t1) n s1
-| TPhide T e t n s :
-    typing T e t n s ->
-    typing T (Ehide e) (Thide t) n (Shide s)
-| TPunhide T e t n s s1 :
-    typing T e (Thide t) n s ->
-    is_hide s = Some s1 ->
-    typing T (Eunhide e) t n s1
-| TPeq T e t1 t2 n s :
-    typing T e t1 n s ->
-    t1 == t2 ->
-    typing T e t2 n s
-| TPsub T e t n n' s s' :
-    typing T e t n s ->
-    n <<= n' ->
-    s <= s' ->
-    typing T e t n' s'
-(* built-in constants *)
-| TPpair T : 
-    typing T Cpair (Tuniversal0 $ Tuniversal0 $ Tarrow #1 F0 Stt $ Tarrow #1 F1 (Spair #1 #0) $ Tprod #3 #2) F0 Stt
-| TPinl T :
-    typing T Cinl (Tuniversal0 $ Tuniversal0 $ Tarrow #1 F1 (Sinl #0) $ Tsum #2 #1) F0 Stt
-| TPinr T :
-    typing T Cinr (Tuniversal0 $ Tuniversal0 $ Tarrow #0 F1 (Sinr #0) $ Tsum #2 #1) F0 Stt
-| TPtt T :
-    typing T Ctt Tunit F0 Stt
-.
-
-(* examples *)
-
-Instance Apply_expr_var_expr : Apply expr var expr :=
-  {
-    apply a b := Eapp a b
-  }.
-
-Instance Apply_type_var_type : Apply type var type :=
-  {
-    apply a b := Tapp a b
-  }.
-
-Lemma Ksum' T a b :
-  kinding T a 0 ->
-  kinding T b 0 ->
-  kinding T (Tsum a b) 0.
-Proof.
-  intros.
-  eapply Kapp.
-  {
-    eapply Kapp.
-    { eapply Ksum. }
-    { eauto. }
-  }
-  { eauto. }
-Qed.
-
-Lemma Kprod' T a b :
-  kinding T a 0 ->
-  kinding T b 0 ->
-  kinding T (Tprod a b) 0.
-Proof.
-  intros.
-  eapply Kapp.
-  {
-    eapply Kapp.
-    { eapply Kprod. }
-    { eauto. }
-  }
-  { eauto. }
-Qed.
 
 Definition Tlist := Tabs $ Trecur $ Tsum Tunit $ Tprod (Thide #1) #0.
 
@@ -363,201 +80,30 @@ Proof.
   }
 Qed.
 
-Lemma Qbeta' t1 t2 t' :
-  t' = subst t2 t1 ->
-  teq (Tapp (Tabs t1) t2) t'.
-Proof.
-  intros; subst; eapply Qbeta; eauto.
-Qed.
-
 Lemma Qlist (t : type) : (Tlist $$ t) == Trecur (Tsum Tunit $ Tprod (Thide (shift t)) #0).
 Proof.
   eapply Qbeta'.
   simpl; eauto.
 Qed.
 
-Lemma TPapp' T e1 e2 ta tb f g n1 n2 s1 s2 t' : 
-  typing T e1 (Tarrow ta f g tb) n1 s1 ->
-  typing T e2 ta n2 s2 ->
-  t' = subst s2 tb ->
-  typing T (Eapp e1 e2) t' (n1 + n2 + F1 + subst s2 f) (subst s2 g).
-Proof.
-  intros; subst; eapply TPapp; eauto.
-Qed.
-
-Lemma TPtapp' T e t2 n s t n' t' :
-  typing T e (Tuniversal (shift n) (shift s) t) n' Stt ->
-  t' = subst t2 t ->
-  typing T (Etapp e t2) t' (n' + F1 + n) s.
-Proof.
-  intros; subst; eapply TPtapp; eauto.
-Qed.
-
-Lemma TPtapp0 T e t2 t n' t' :
-  typing T e (Tuniversal F0 Stt t) n' Stt ->
-  t' = subst t2 t ->
-  typing T (Etapp e t2) t' (n' + F1 + F0) Stt.
-Proof.
-  intros; subst; eapply TPtapp'; eauto.
-Qed.
-
-Lemma TPvar' T n t s t' s' : 
-  find n T = Some (TEtyping (t, s)) -> 
-  t' = shiftby (S n) t ->
-  s' = default (var_to_size #n) (shiftby (S n) s) ->
-  typing T #n t' F0 s'.
-Proof.
-  intros; subst; eapply TPvar; eauto.
-Qed.
-
-Lemma TPweaken T T' e t n s T'' :
-  typing T e t n s ->
-  T'' = T ++ T' ->
-  typing T'' e t n s.
-Proof.
-  admit.
-Qed.
-
-Lemma TPweaken_empty T e t n s :
-  typing [] e t n s ->
-  typing T e t n s.
-Proof.
-  intros H.
-  eapply TPweaken; eauto.
-  simpl; eauto.
-Qed.
-
 Arguments compose / . 
 Arguments flip / . 
-Arguments add_typing / . 
-Arguments add_typings / . 
-Arguments add_kinding / . 
 
-Arguments Tprod / .
+Close Scope F01.
 
-Arguments add_snd {A B} b a / .
-
-Lemma TPunfold' T e t n s s1 t1 t' :
-  typing T e t n s ->
-  is_fold s = Some s1 ->
-  t == Trecur t1 ->
-  t' = subst t t1 ->
-  typing T (Eunfold t e) t' n s1.
-Proof.
-  intros; subst; eapply TPunfold; eauto.
-Qed.
-
-Lemma TPmatch_pair' T e e' t t1 t2 n s n' s' s1 s2 t'' s'' :
-  typing T e (Tprod t1 t2) n s ->
-  is_pair s = Some (s1, s2) ->
-  let t12 := [(t1, Some s1); (t2, Some s2)] in
-  let T' := add_typings t12 T in
-  typing T' e' t n' s' ->
-  let s12 := [s1; s2] in
-  t'' = subst_list s12 t ->
-  s'' = subst_list s12 s' ->
-  typing T (Ematch_pair e e') t'' (n + F1 + subst_list s12 n') s''.
-Proof.
-  intros; subst; eapply TPmatch_pair; eauto.
-Qed.
-
-Lemma TPpair_app T A B a b n1 n2 s1 s2 :
-  typing T a A n1 s1 ->
-  typing T b B n2 s2 ->
-  typing T (Epair $$ A $$ B $$ a $$ b) (Tprod A B) (n1 + n2 + F1) (Spair s1 s2).
-Proof.
-  intros Ha Hb.
-  eapply TPsub.
+Instance Apply_expr_var_expr : Apply expr var expr :=
   {
-    eapply TPapp'.
-    {
-      eapply TPapp'.
-      {
-        eapply TPtapp0.
-        {
-          eapply TPtapp0.
-          { eapply TPpair. }
-          { simpl; eauto. }
-        }
-        { simpl; eauto. }
-      }
-      {
-        repeat rewrite fold_subst_t_t in *.
-        repeat rewrite fold_shift_from_t in *.
-        repeat rewrite subst_shift_t_t in *.
-        eauto.
-      }
-      { simpl; eauto. }
-    }
-    {
-      repeat rewrite fold_subst_s_t in *.
-      repeat rewrite fold_shift_from_t in *.
-      repeat rewrite subst_shift_s_t in *.
-      eauto.
-    }
-    {
-      simpl.
-      repeat rewrite fold_subst_s_t in *.
-      repeat rewrite fold_shift_from_t in *.
-      fold (iter 2 (shift_from_t 0) B).
-      repeat rewrite subst_shift_s_t_n in *.
-      simpl.
-      repeat rewrite fold_subst_s_t in *.
-      repeat rewrite fold_shift_from_t in *.
-      repeat rewrite subst_shift_s_t in *.
-      eauto. 
+    apply a b := Eapp a b
+  }.
 
-      simpl. 
-      repeat rewrite fold_shift_from_t in *.
-      repeat rewrite fold_subst_s_t in *.
-      fold (iter 3 (shift_from_t 0) A).
-      repeat rewrite subst_shift_t_t_n in *.
-      simpl.
-      repeat rewrite fold_subst_s_t in *.
-      repeat rewrite fold_shift_from_t in *.
-      fold (iter 2 (shift_from_t 0) A).
-      repeat rewrite subst_shift_s_t_n in *.
-      simpl.
-      repeat rewrite fold_subst_s_t in *.
-      repeat rewrite fold_shift_from_t in *.
-      repeat rewrite subst_shift_s_t in *.
-      eauto. 
-    }
-  }
+Instance Apply_type_var_type : Apply type var type :=
   {
-    simpl.
-    leO_solver.
-  }
-  {
-    simpl.
-    repeat rewrite fold_subst_s_s in *.
-    repeat rewrite fold_shift_from_s in *.
-    repeat rewrite subst_shift_s_s in *.
-    reflexivity.
-  }
-Qed.
+    apply a b := Tapp a b
+  }.
 
 Definition Eunhide_fst := Etabs $ Etabs $ Eabs (Tprod (Thide #1) #0) $ 
                                      Ematch_pair #0 $
                                      Epair $$ (#4 : type) $$ (#3 : type) $$ (Eunhide #1) $$ #0.
-
-Lemma TPsubn T e t n s n' :
-  typing T e t n s ->
-  n <<= n' ->
-  typing T e t n' s.
-Proof.
-  intros; eapply TPsub; eauto.
-  reflexivity.
-Qed.
-
-Close Scope F01.
-
-Lemma TPtabs0 T e t :
-  typing (add_kinding 0 T) e t F0 Stt ->
-  typing T (Etabs e) (Tuniversal F0 Stt t) F0 Stt.
-Proof.
-  intros; eapply TPtabs with (n := F0) (s := Stt); simpl; eauto.
-Qed.
 
 Lemma TPunhide_fst :
   typing [] Eunhide_fst (Tuniversal0 $ Tuniversal0 $ Tarrow (Tprod (Thide #1) #0) F1 (Spair (Svar (#0, [Punhide; Pfst])) (Svar (#0, [Psnd]))) $ Tprod #2 #1) F0 Stt.
@@ -666,96 +212,6 @@ Definition Econs :=
         let telm := #2 : type in
         let tlist := Tlist $ telm in
         Efold tlist (Einr $$ Tunit $$ Tprod (Thide telm) tlist $$ (Epair $$ Thide telm $$ tlist $$ Ehide #1 $$ #0)).
-
-Lemma TPinl_app T A B e n s :
-  typing T e A n s ->
-  typing T (Einl $$ A $$ B $$ e) (Tsum $$ A $$ B) (n + F1) (Sinl s).
-Proof.
-  intros H.
-  eapply TPsub.
-  {
-    eapply TPapp'.
-    {
-      eapply TPtapp0.
-      {
-        eapply TPtapp0.
-        { eapply TPinl. }
-        { simpl; eauto. }
-      }              
-      { simpl; eauto. }
-    }
-    { 
-      simpl.
-      repeat rewrite fold_shift_from_t in *.
-      repeat rewrite fold_subst_t_t in *.
-      repeat rewrite subst_shift_t_t in *.
-      eauto.
-    }
-    { 
-      simpl.
-      repeat rewrite fold_shift_from_t in *.
-      repeat rewrite fold_subst_s_t in *.
-      repeat rewrite subst_shift_s_t in *.
-      fold (iter 2 (shift_from_t 0) A).
-      repeat rewrite subst_shift_t_t_n in *.
-      simpl.
-      repeat rewrite fold_shift_from_t in *.
-      repeat rewrite fold_subst_s_t in *.
-      repeat rewrite subst_shift_s_t in *.
-      eauto.
-    }
-  }
-  {
-    simpl.
-    leO_solver.
-  }
-  {
-    simpl.
-    reflexivity.
-  }
-Qed.
-
-Lemma TPinr_app T A B e n s :
-  typing T e B n s ->
-  typing T (Einr $$ A $$ B $$ e) (Tsum $$ A $$ B) (n + F1) (Sinr s).
-Proof.
-  intros H.
-  eapply TPsub.
-  {
-    eapply TPapp'.
-    {
-      eapply TPtapp0.
-      {
-        eapply TPtapp0.
-        { eapply TPinr. }
-        { simpl; eauto. }
-      }              
-      { simpl; eauto. }
-    }
-    { eauto. }          
-    { 
-      simpl.
-      repeat rewrite fold_shift_from_t in *.
-      repeat rewrite fold_subst_s_t in *.
-      repeat rewrite subst_shift_s_t in *.
-      fold (iter 2 (shift_from_t 0) A).
-      repeat rewrite subst_shift_t_t_n in *.
-      simpl.
-      repeat rewrite fold_shift_from_t in *.
-      repeat rewrite fold_subst_s_t in *.
-      repeat rewrite subst_shift_s_t in *.
-      eauto.
-    }
-  }
-  {
-    simpl.
-    leO_solver.
-  }
-  {
-    simpl.
-    reflexivity.
-  }
-Qed.
 
 Lemma TPnil :
   typing [] Enil (Tuniversal F1 (Sfold (Sinl Stt)) $ Tlist $$ #0) F0 Stt.
@@ -922,15 +378,6 @@ Definition is_list s :=
   s1 <- is_hide s1 ;;
   ret (s1, s2).
 
-Lemma TPsubs T e t n s s' :
-  typing T e t n s ->
-  s <= s' ->
-  typing T e t n s'.
-Proof.
-  intros; eapply TPsub; eauto.
-  reflexivity.
-Qed.
-
 Lemma is_list_elim s p : is_list s = Some p -> exists s1 s2 s3 s4, is_fold s = Some s1 /\ is_inlinr s1 = Some (s2, s3) /\ is_pair s3 = Some (s4, snd p) /\ is_hide s4 = Some (fst p).
 Proof.
   intros H.
@@ -956,304 +403,7 @@ Proof.
   }
 Qed.
 
-Lemma is_pair_shift sp s1 s2 : is_pair sp = Some (s1, s2) -> is_pair (shift sp) = Some (shift s1, shift s2).
-Proof.
-  destruct sp; simpl; try discriminate; intros H; inject H; eauto.
-  destruct x.
-  eauto.
-Qed.
-
-Lemma is_hide_shift s s' : is_hide s = Some s' -> is_hide (shift s) = Some (shift s').
-Proof.
-  destruct s; simpl; try discriminate; intros H; inject H; eauto.
-  destruct x.
-  eauto.
-Qed.
-
 Definition removen A n ls := @firstn A n ls ++ skipn (S n) ls.
-
-Definition shift_from_TE n te :=
-  match te with
-    | TEtyping ty => TEtyping $ shift_from n ty
-    | TEkinding k => te
-  end.
-
-Instance Shift_tc_entry : Shift tc_entry :=
-  {
-    shift_from := shift_from_TE
-  }.
-
-Lemma Kshift a T t k : kinding T t k -> kinding (a :: T) (shift t) k.
-  admit.
-Qed.
-
-Lemma fold_shift_from_e n x : visit_e n (shift_e_f, shift_from) x = shift_from_e n x.
-Proof.
-  eauto.
-Qed.
-
-Definition uncurry {U V W : Type} (f : U -> V -> W) (p : U*V) : W :=
-  f (fst p) (snd p).
-Arguments uncurry {U V W} f p / .
-
-Fixpoint rev_range len :=
-  match len with
-    | 0 => nil
-    | S n => n :: rev_range n
-  end.
-
-Open Scope F.
-
-Lemma subst_shift_from_s_t x : forall v n m, (m <= n)%nat -> subst_size_type m (shift_from_s n v) (shift_from_t (S n) x) = shift_from_t n (subst_size_type m v x).
-  admit.
-Qed.
-Lemma subst_shift_from_s_s x : forall v n m, (m <= n)%nat -> subst_size_size m (shift_from_s n v) (shift_from_s (S n) x) = shift_from_s n (subst_size_size m v x).
-  admit.
-Qed.
-Lemma subst_shift_from_t_t x : forall v n m, (m <= n)%nat -> subst_t_t m (shift_from_t n v) (shift_from_t (S n) x) = shift_from_t n (subst_t_t m v x).
-  admit.
-Qed.
-Lemma shift_from_shift_from_f x n : shift_from_f (S n) (shift_from_f 0 x) = shift_from_f 0 (shift_from_f n x).
-  admit.
-Qed.
-Lemma shift_from_shift_from_s x n : shift_from_s (S n) (shift_from_s 0 x) = shift_from_s 0 (shift_from_s n x).
-  admit.
-Qed.
-Lemma Kinsert T t k : 
-  kinding T t k ->
-  forall T1 skipped T2 T' m,
-    T = T1 ++ T2 ->
-    m = length T1 ->
-    T' = map (uncurry shift_from) (combine (rev_range m) T1) ++ skipped :: T2 ->
-    kinding T' (shift_from m t) k.
-  admit.
-Qed.
-
-Lemma TPlet' T t1 e1 e2 t2 n1 n2 s1 s2 t2' :
-  typing T e1 t1 n1 s1 ->
-  typing (add_typing (t1, Some s1) T) e2 t2 n2 s2 ->
-  t2' = subst s1 t2 ->
-  typing T (Elet t1 e1 e2) t2' (n1 + subst s1 n2) (subst s1 s2).
-Proof.
-  intros; subst; eapply TPlet; eauto.
-Qed.
-
-Lemma TPinsert T e t c s : 
-  typing T e t c s ->
-  forall T1 skipped T2 T' m,
-    T = T1 ++ T2 ->
-    m = length T1 ->
-    T' = map (uncurry shift_from) (combine (rev_range m) T1) ++ skipped :: T2 ->
-    typing T' (shift_from m e) (shift_from m t) (shift_from m c) (shift_from m s).
-Proof.
-  induction 1.
-  {
-    unfold_all; intros T1 skipped T2 T' m ? ? ?; subst.
-    rename n into x.
-    Arguments shift_e_f nv nq / .
-    simpl in *.
-    repeat rewrite fold_shift_from_t in *.
-    repeat rewrite fold_shift_from_s in *.
-    destruct (nat_cmp x (length T1)) as [x' ? Hc | ? | x' ? Hc]; subst.
-    {
-      eapply TPvar'.
-      { simpl.
-        rewrite Expr.nth_error_app_L in H by eauto.
-        eapply Structured.nth_error_app1.
-        etransitivity.
-        {
-          eapply map_nth_error.
-          eapply nth_error_combine.
-          {
-            Lemma nth_error_rev_range len i : i < len -> nth_error (rev_range len) i = Some (len - (1 + i)).
-              admit.
-            Qed.
-            rewrite nth_error_rev_range by eauto.
-            eauto.
-          }
-          { eauto. }
-        }
-        { simpl; eauto. }
-      }
-      { simpl.
-        admit.
-      }
-      admit.
-    }
-    admit.
-    admit.
-  }
-  {
-    unfold_all; intros T1 skipped T2 T' m ? ? ?; subst.
-    simpl in *.
-    repeat rewrite fold_shift_from_s in *.
-    repeat rewrite fold_subst_s_f in *.
-    repeat rewrite fold_shift_from_f in *.
-    repeat rewrite <- subst_shift_from_s_f by omega.
-    repeat rewrite fold_subst_s_s in *.
-    repeat rewrite <- subst_shift_from_s_s by omega.
-    eapply TPapp'.
-    { eapply IHtyping1; eauto. }
-    { eapply IHtyping2; eauto. }
-    simpl.
-    repeat rewrite fold_shift_from_t in *.
-    repeat rewrite fold_subst_s_t in *.
-    repeat rewrite fold_shift_from_s in *.
-    repeat rewrite subst_shift_s_t in *.
-    repeat rewrite subst_shift_from_s_t by omega.
-    eauto.
-  }
-  {
-    unfold_all; intros T1 skipped T2 T' m ? ? ?; subst.
-    simpl in *.
-    eapply TPabs.
-    { eapply Kinsert; eauto. }
-    eapply IHtyping. 
-    { rewrite app_comm_cons.
-      eauto.
-    }
-    { eauto. }
-    { simpl; eauto. }
-  }
-  {
-    unfold_all; intros T1 skipped T2 T' m ? ? ?; subst.
-    simpl in *.
-    eapply TPtapp'.
-    { simpl. 
-      repeat rewrite fold_shift_from_e in *.
-      repeat rewrite fold_shift_from_s in *.
-      repeat rewrite fold_shift_from_f in *.
-      repeat rewrite <- shift_from_shift_from_f in *.
-      repeat rewrite <- shift_from_shift_from_s in *.
-      { eapply IHtyping; eauto. }
-    }
-    simpl.
-    repeat rewrite fold_shift_from_t in *.
-    repeat rewrite fold_subst_t_t in *.
-    repeat rewrite subst_shift_from_t_t by omega.
-    eauto.
-  }
-  {
-    unfold_all; intros T1 skipped T2 T' m ? ? ?; subst.
-    simpl in *.
-    eapply TPtabs.
-    eapply IHtyping. 
-    { rewrite app_comm_cons.
-      eauto.
-    }
-    { eauto. }
-    { simpl; eauto. }
-  }
-  {
-    unfold_all; intros T1 skipped T2 T' m ? ? ?; subst.
-    simpl in *.
-    repeat rewrite fold_shift_from_s in *.
-    repeat rewrite fold_subst_s_f in *.
-    repeat rewrite fold_shift_from_f in *.
-    repeat rewrite <- subst_shift_from_s_f by omega.
-    repeat rewrite fold_subst_s_s in *.
-    repeat rewrite <- subst_shift_from_s_s by omega.
-    eapply TPlet'.
-    { eapply IHtyping1; eauto. }
-    { eapply IHtyping2.
-      { rewrite app_comm_cons.
-        eauto.
-      }
-      { eauto. }
-      { simpl; eauto. }
-    }
-    simpl.
-    repeat rewrite fold_shift_from_t in *.
-    repeat rewrite fold_subst_s_t in *.
-    repeat rewrite fold_shift_from_s in *.
-    repeat rewrite subst_shift_s_t in *.
-    repeat rewrite subst_shift_from_s_t by omega.
-    eauto.
-  }
-  {
-(*
-    unfold_all; intros T1 skipped T2 T' m ? ? ?; subst.
-    simpl.
-    eapply TPletrec.
-    {
-      intros lhs_t rhs_t e Hin.
-      Lemma in_loop A B ls b f : In b ((fix loop (ls : list A) : list B := match ls with [] => [] | x :: xs => f x :: loop xs end) ls) -> exists a, In a ls /\ f a = b.
-        admit.
-      Qed.
-      (*here*)
-      eapply (@in_loop (type * type * expr) (type * type * expr)) in Hin.
-    }
-    repeat rewrite fold_shift_from_s in *.
-    repeat rewrite fold_subst_s_f in *.
-    repeat rewrite fold_shift_from_f in *.
-    repeat rewrite <- subst_shift_from_s_f by omega.
-    repeat rewrite fold_subst_s_s in *.
-    repeat rewrite <- subst_shift_from_s_s by omega.
-    eapply TPlet'.
-    { eapply IHtyping1; eauto. }
-    { eapply IHtyping2.
-      { rewrite app_comm_cons.
-        eauto.
-      }
-      { eauto. }
-      { simpl; eauto. }
-    }
-    simpl.
-    repeat rewrite fold_shift_from_t in *.
-    repeat rewrite fold_subst_s_t in *.
-    repeat rewrite fold_shift_from_s in *.
-    repeat rewrite subst_shift_s_t in *.
-    repeat rewrite subst_shift_from_s_t by omega.
-    eauto.
-*)
-    admit.
-  }
-
-  admit.
-  admit.
-  admit.
-  admit.
-  admit.
-  admit.
-  admit.
-  admit.
-  admit.
-  admit.
-  admit.
-  admit.
-  admit.
-  admit.
-Qed.
-
-Lemma TPinsert2 T e t n s r0 r1 r2 r0' r1' : 
-  typing (r0 :: r1 :: T) e t n s ->
-  r0' = shift_from 1 r0 ->
-  r1' = shift_from 0 r1 ->
-  typing (r0' :: r1' :: r2 :: T) (shift_from 2 e) (shift_from 2 t) (shift_from 2 n) (shift_from 2 s).
-Proof.
-  intros H ? ?; subst.
-  eapply TPinsert; eauto.
-  {
-    instantiate (1 := T).
-    instantiate (1 := [r0; r1]).
-    eauto.
-  }
-  { eauto. }
-  simpl; eauto.
-Qed.
-
-Lemma TPinsert0 T e t n s r : typing T e t n s -> typing (r :: T) (shift e) (shift t) (shift n) (shift s).
-Proof.
-  intros H.
-  eapply TPinsert; eauto.
-  {
-    instantiate (1 := T).
-    instantiate (1 := []).
-    eauto.
-  }
-  { eauto. }
-  simpl; eauto.
-Qed.
 
 Lemma TPmatch_list T e e1 e2 telm n s s1 s2 t' na nb s' :
   let list := Tlist $ telm in
@@ -2044,13 +1194,16 @@ Definition nostuck e := forall e', steps e e' -> IsValue e' \/ exists e'', step 
 
 Theorem type_soundness : forall t1 c s e t, 
   typing [TEtyping (t1, None)] e t c s -> 
+  (forall v1,
+     IsValue v1 ->
+     typingsim [] v1 t1 ->
+     nostuck (subst v1 e)) /\
   exists Ct s0, 
     forall v1,
       IsValue v1 ->
       typingsim [] v1 t1 ->
       let s1 := get_size v1 in
       (s0 <= s1) ->
-      nostuck (subst v1 e) /\
       forall v n, 
         IsValue v -> 
         nsteps (subst v1 e) n v ->
