Syntax.v
@@ -1,4 +1,5 @@
 Require Import Complexity.
+
 Export Complexity.
 
 Inductive tconstr :=
