Typing.v
@@ -1,0 +1,247 @@
+Set Implicit Arguments.
+Unset Strict Implicit.
+Unset Printing Implicit Defensive. 
+Generalizable All Variables.
+
+Require Import List.
+Require Import Program.
+Require Import Util.
+Require Import Syntax.
+Require Import Subst.
+Require Import Order.
+
+Export Syntax Subst Order.
+
+Import ListNotations.
+Open Scope list_scope.
+
+Instance Shift_option `{Shift A} : Shift (option A) :=
+  {
+    shift_from n o := option_map (shift_from n) o
+  }.
+
+Instance Shift_pair `{Shift A, Shift B} : Shift (A * B) :=
+  {
+    shift_from n p := (shift_from n (fst p), shift_from n (snd p))
+  }.
+
+(* kinds are restricted to the form (* => * => ... => *). 0 means * *)
+Definition kind := nat.
+
+(* Typing context.
+   The second field of TEtyping is the optional size constraint
+ *)
+Inductive tc_entry := 
+  | TEtyping (_ : type * option size)
+  | TEkinding (_ : kind).
+
+Definition tcontext := list tc_entry.
+
+Definition add_typing t T := TEtyping t :: T.
+Definition add_typings ls T := fst $ fold_left (fun (p : tcontext * nat) t => let (T, n) := p in (add_typing (shiftby n t) T, S n)) ls (T, 0%nat).
+Definition add_kinding k T := TEkinding k :: T.
+
+Coercion var_to_size (x : var) : size := Svar (x, []).
+
+Class Find key value container := 
+  {
+    find : key -> container -> option value
+  }.
+
+Instance Find_list A : Find nat A (list A) :=
+  {
+    find k c := @nth_error A c k
+  }.
+
+Close Scope F01.
+
+Inductive kinding : tcontext -> type -> kind -> Prop :=
+| Kvar T n k : find n T = Some (TEkinding k) -> kinding T #n k
+| Kapp T t1 t2 k :
+    kinding T t1 (S k) ->
+    kinding T t2 0 ->
+    kinding T (Tapp t1 t2) k
+| Kabs T t k :
+    kinding (add_kinding 0 T) t k ->
+    kinding T (Tabs t) (S k)
+| Karrow T t1 f g t2 :
+    kinding T t1 0 ->
+    kinding (add_typing (t1, None) T) t2 0 ->
+    kinding T (Tarrow t1 f g t2) 0
+| Kuniversal T f g t :
+    kinding (add_kinding 0 T) t 0 ->
+    kinding T (Tuniversal f g t) 0
+| Krecur T t :
+    kinding (add_kinding 0 T) t 0 ->
+    kinding T (Trecur t) 0
+| Khide T t :
+    kinding T t 0 ->
+    kinding T (Thide t) 0
+| Kunit T :
+    kinding T (Tconstr TCunit) 0
+| Kprod T :
+    kinding T (Tconstr TCprod) 2
+| Ksum T :
+    kinding T (Tconstr TCsum) 2
+.
+
+Inductive teq : type -> type -> Prop :=
+| Qrefl t : teq t t
+| Qsymm a b : teq a b -> teq b a
+| Qtrans a b c : teq a b -> teq b c -> teq a c
+| Qabs a b :
+    teq a b ->
+    teq (Tabs a) (Tabs b)
+| Qapp a b a' b' :
+    teq a a' ->
+    teq b b' ->
+    teq (Tapp a b) (Tapp a' b')
+| Qbeta t1 t2 :
+    teq (Tapp (Tabs t1) t2) (subst t2 t1)
+| Qarrow a f g b a' b' : 
+    teq a a' ->
+    teq b b' ->
+    teq (Tarrow a f g b) (Tarrow a' f g b')
+| Qrecur a b :
+    teq a b ->
+    teq (Trecur a) (Trecur b)
+.
+
+Global Add Relation type teq
+    reflexivity proved by Qrefl
+    symmetry proved by Qsymm
+    transitivity proved by Qtrans
+      as teq_rel.
+
+Class Equal t :=
+  {
+    equal : t -> t -> Prop
+  }.
+
+Infix "==" := equal (at level 70) : G.
+
+Instance Equal_type : Equal type :=
+  {
+    equal := teq
+  }.
+
+Definition add_snd {A B} (b : B) (a : A) := (a, b).
+
+Open Scope F.
+Open Scope G.
+
+Infix "<<" := compose (at level 40) : prog_scope.
+Infix ">>" := (flip compose) (at level 40) : prog_scope.
+Open Scope prog_scope.
+
+Instance Apply_type_type_type : Apply type type type :=
+  {
+    apply := Tapp
+  }.
+
+Instance Apply_expr_expr_expr : Apply expr expr expr :=
+  {
+    apply := Eapp
+  }.
+
+Instance Apply_expr_type_expr : Apply expr type expr :=
+  {
+    apply := Etapp
+  }.
+
+Definition Tunit := Tconstr TCunit.
+Definition Tprod t1 t2 := Tconstr TCprod $$ t1 $$ t2.
+Definition Tsum t1 t2 := Tconstr TCsum $$ t1 $$ t2.
+
+Notation Tuniversal0 := (Tuniversal F0 Stt).
+
+Inductive typing : tcontext -> expr -> type -> cexpr -> size -> Prop :=
+| TPvar T n t s : 
+    find n T = Some (TEtyping (t, s)) -> 
+    typing T #n (shiftby (S n) t) F0 (default (var_to_size #n) (shiftby (S n) s))
+| TPapp T e1 e2 ta tb n s n1 n2 nouse s2 : 
+    typing T e1 (Tarrow ta n s tb) n1 nouse ->
+    typing T e2 ta n2 s2 ->
+    typing T (Eapp e1 e2) (subst s2 tb) (n1 + n2 + F1 + subst s2 n) (subst s2 s)
+| TPabs T e t1 t2 n s :
+    kinding T t1 0 ->
+    typing (add_typing (t1, None) T) e t2 n s ->
+    typing T (Eabs t1 e) (Tarrow t1 n s t2) F0 Stt
+| TPtapp T e t2 n s t n' :
+    typing T e (Tuniversal (shift n) (shift s) t) n' Stt ->
+    typing T (Etapp e t2) (subst t2 t) (n' + F1 + n) s
+| TPtabs T e n s t :
+    typing (add_kinding 0 T) e t n s ->
+    typing T (Etabs e) (Tuniversal n s t) F0 Stt
+| TPlet T t1 e1 e2 t2 n1 n2 s1 s2:
+    typing T e1 t1 n1 s1 ->
+    typing (add_typing (t1, Some s1) T) e2 t2 n2 s2 ->
+    typing T (Elet t1 e1 e2) (subst s1 t2) (n1 + subst s1 n2) (subst s1 s2)
+| TPletrec T (defs : list letrec_entry) main t n s :
+    let len := length defs in
+    let T' := add_typings (map (fst >> fst >> add_snd (Some Stt)) defs) T in
+    (forall lhs_t rhs_t e, 
+       In (lhs_t, rhs_t, e) defs -> 
+       typing T' (Eabs rhs_t e) (shiftby len lhs_t) F0 Stt) ->
+    typing T' main (shiftby len t) (shiftby len n) (shiftby len s) ->
+    typing T (Eletrec defs main) t n s
+| TPmatch_pair T e e' t t1 t2 n s n' s' s1 s2 :
+    typing T e (Tprod t1 t2) n s ->
+    is_pair s = Some (s1, s2) ->
+    let t12 := [(t1, Some s1); (t2, Some s2)] in
+    let T' := add_typings t12 T in
+    typing T' e' t n' s' ->
+    let s12 := [s1; s2] in
+    typing T (Ematch_pair e e') (subst_list s12 t) (n + F1 + subst_list s12 n') (subst_list s12 s')
+| TPmatch_inlinr T e e1 e2 t1 t2 n s s1 s2 t n1 n2 s' :
+    typing T e (Tsum t1 t2) n s ->
+    is_inlinr s = Some (s1, s2) ->
+    (* timing constraints are passed forward; size and type constraints are passed backward.
+       t' and s' are backward guidance for branches *)
+    typing (add_typing (t1, Some s1) T) e1 (shift t) n1 (shift s') -> 
+    typing (add_typing (t2, Some s2) T) e2 (shift t) n2 (shift s') -> 
+    typing T (Ematch_sum e e1 e2) t (n + F1 + max (subst s1 n1) (subst s2 n2)) s'
+| TPmatch_inl T e e1 e2 t1 t2 n s t' n' s' :
+    typing T e (Tsum t1 t2) n (Sinl s) ->
+    typing (add_typing (t1, Some s) T) e1 t' n' s' ->
+    typing T (Ematch_sum e e1 e2) (subst s t') (n + F1 + subst s n') (subst s s')
+| TPmatch_inr T e e1 e2 t1 t2 n s t' n' s' :
+    typing T e (Tsum t1 t2) n (Sinr s) ->
+    typing (add_typing (t2, Some s) T) e2 t' n' s' ->
+    typing T (Ematch_sum e e1 e2) (subst s t') (n + F1 + subst s n') (subst s s')
+| TPfold T e t n s t1 :
+    t == Trecur t1 ->
+    typing T e (subst t t1) n s ->
+    typing T (Efold t e) t n (Sfold s)
+| TPunfold T e t n s s1 t1 :
+    typing T e t n s ->
+    is_fold s = Some s1 ->
+    t == Trecur t1 ->
+    typing T (Eunfold t e) (subst t t1) n s1
+| TPhide T e t n s :
+    typing T e t n s ->
+    typing T (Ehide e) (Thide t) n (Shide s)
+| TPunhide T e t n s s1 :
+    typing T e (Thide t) n s ->
+    is_hide s = Some s1 ->
+    typing T (Eunhide e) t n s1
+| TPeq T e t1 t2 n s :
+    typing T e t1 n s ->
+    t1 == t2 ->
+    typing T e t2 n s
+| TPsub T e t n n' s s' :
+    typing T e t n s ->
+    n <<= n' ->
+    s <= s' ->
+    typing T e t n' s'
+(* built-in constants *)
+| TPpair T : 
+    typing T Cpair (Tuniversal0 $ Tuniversal0 $ Tarrow #1 F0 Stt $ Tarrow #1 F1 (Spair #1 #0) $ Tprod #3 #2) F0 Stt
+| TPinl T :
+    typing T Cinl (Tuniversal0 $ Tuniversal0 $ Tarrow #1 F1 (Sinl #0) $ Tsum #2 #1) F0 Stt
+| TPinr T :
+    typing T Cinr (Tuniversal0 $ Tuniversal0 $ Tarrow #0 F1 (Sinr #0) $ Tsum #2 #1) F0 Stt
+| TPtt T :
+    typing T Ctt Tunit F0 Stt
+.
+
