TypingFacts.v
@@ -1,0 +1,627 @@
+Require Import List.
+Require Import Bedrock.Platform.Cito.GeneralTactics3.
+Require Import Bedrock.Platform.Cito.GeneralTactics4.
+Require Import Bedrock.Expr.
+Require Import Bedrock.Structured.
+Require Import Bedrock.Platform.Cito.ListFacts4.
+Require Import Util.
+Require Import Typing.
+
+Export Typing.
+
+Import ListNotations.
+Open Scope list_scope.
+
+Lemma Ksum' T a b :
+  kinding T a 0 ->
+  kinding T b 0 ->
+  kinding T (Tsum a b) 0.
+Proof.
+  intros.
+  eapply Kapp.
+  {
+    eapply Kapp.
+    { eapply Ksum. }
+    { eauto. }
+  }
+  { eauto. }
+Qed.
+
+Lemma Kprod' T a b :
+  kinding T a 0 ->
+  kinding T b 0 ->
+  kinding T (Tprod a b) 0.
+Proof.
+  intros.
+  eapply Kapp.
+  {
+    eapply Kapp.
+    { eapply Kprod. }
+    { eauto. }
+  }
+  { eauto. }
+Qed.
+
+Lemma Qbeta' t1 t2 t' :
+  t' = subst t2 t1 ->
+  teq (Tapp (Tabs t1) t2) t'.
+Proof.
+  intros; subst; eapply Qbeta; eauto.
+Qed.
+
+Lemma TPapp' T e1 e2 ta tb f g n1 n2 s1 s2 t' : 
+  typing T e1 (Tarrow ta f g tb) n1 s1 ->
+  typing T e2 ta n2 s2 ->
+  t' = subst s2 tb ->
+  typing T (Eapp e1 e2) t' (n1 + n2 + F1 + subst s2 f) (subst s2 g).
+Proof.
+  intros; subst; eapply TPapp; eauto.
+Qed.
+
+Lemma TPtapp' T e t2 n s t n' t' :
+  typing T e (Tuniversal (shift n) (shift s) t) n' Stt ->
+  t' = subst t2 t ->
+  typing T (Etapp e t2) t' (n' + F1 + n) s.
+Proof.
+  intros; subst; eapply TPtapp; eauto.
+Qed.
+
+Lemma TPtapp0 T e t2 t n' t' :
+  typing T e (Tuniversal F0 Stt t) n' Stt ->
+  t' = subst t2 t ->
+  typing T (Etapp e t2) t' (n' + F1 + F0) Stt.
+Proof.
+  intros; subst; eapply TPtapp'; eauto.
+Qed.
+
+Lemma TPvar' T n t s t' s' : 
+  find n T = Some (TEtyping (t, s)) -> 
+  t' = shiftby (S n) t ->
+  s' = default (var_to_size #n) (shiftby (S n) s) ->
+  typing T #n t' F0 s'.
+Proof.
+  intros; subst; eapply TPvar; eauto.
+Qed.
+
+Lemma TPweaken T T' e t n s T'' :
+  typing T e t n s ->
+  T'' = T ++ T' ->
+  typing T'' e t n s.
+Proof.
+  admit.
+Qed.
+
+Lemma TPweaken_empty T e t n s :
+  typing [] e t n s ->
+  typing T e t n s.
+Proof.
+  intros H.
+  eapply TPweaken; eauto.
+  simpl; eauto.
+Qed.
+
+Arguments add_typing / . 
+Arguments add_typings / . 
+Arguments add_kinding / . 
+
+Arguments Tprod / .
+
+Arguments add_snd {A B} b a / .
+
+Lemma TPunfold' T e t n s s1 t1 t' :
+  typing T e t n s ->
+  is_fold s = Some s1 ->
+  t == Trecur t1 ->
+  t' = subst t t1 ->
+  typing T (Eunfold t e) t' n s1.
+Proof.
+  intros; subst; eapply TPunfold; eauto.
+Qed.
+
+Lemma TPmatch_pair' T e e' t t1 t2 n s n' s' s1 s2 t'' s'' :
+  typing T e (Tprod t1 t2) n s ->
+  is_pair s = Some (s1, s2) ->
+  let t12 := [(t1, Some s1); (t2, Some s2)] in
+  let T' := add_typings t12 T in
+  typing T' e' t n' s' ->
+  let s12 := [s1; s2] in
+  t'' = subst_list s12 t ->
+  s'' = subst_list s12 s' ->
+  typing T (Ematch_pair e e') t'' (n + F1 + subst_list s12 n') s''.
+Proof.
+  intros; subst; eapply TPmatch_pair; eauto.
+Qed.
+
+Definition Epair := Econstr Cpair.
+Definition Einl := Econstr Cinl.
+Definition Einr := Econstr Cinr.
+Definition Ett := Econstr Ctt.
+
+Lemma TPpair_app T A B a b n1 n2 s1 s2 :
+  typing T a A n1 s1 ->
+  typing T b B n2 s2 ->
+  typing T (Epair $$ A $$ B $$ a $$ b) (Tprod A B) (n1 + n2 + F1) (Spair s1 s2).
+Proof.
+  intros Ha Hb.
+  eapply TPsub.
+  {
+    eapply TPapp'.
+    {
+      eapply TPapp'.
+      {
+        eapply TPtapp0.
+        {
+          eapply TPtapp0.
+          { eapply TPpair. }
+          { simpl; eauto. }
+        }
+        { simpl; eauto. }
+      }
+      {
+        repeat rewrite fold_subst_t_t in *.
+        repeat rewrite fold_shift_from_t in *.
+        repeat rewrite subst_shift_t_t in *.
+        eauto.
+      }
+      { simpl; eauto. }
+    }
+    {
+      repeat rewrite fold_subst_s_t in *.
+      repeat rewrite fold_shift_from_t in *.
+      repeat rewrite subst_shift_s_t in *.
+      eauto.
+    }
+    {
+      simpl.
+      repeat rewrite fold_subst_s_t in *.
+      repeat rewrite fold_shift_from_t in *.
+      fold (iter 2 (shift_from_t 0) B).
+      repeat rewrite subst_shift_s_t_n in *.
+      simpl.
+      repeat rewrite fold_subst_s_t in *.
+      repeat rewrite fold_shift_from_t in *.
+      repeat rewrite subst_shift_s_t in *.
+      eauto. 
+
+      simpl. 
+      repeat rewrite fold_shift_from_t in *.
+      repeat rewrite fold_subst_s_t in *.
+      fold (iter 3 (shift_from_t 0) A).
+      repeat rewrite subst_shift_t_t_n in *.
+      simpl.
+      repeat rewrite fold_subst_s_t in *.
+      repeat rewrite fold_shift_from_t in *.
+      fold (iter 2 (shift_from_t 0) A).
+      repeat rewrite subst_shift_s_t_n in *.
+      simpl.
+      repeat rewrite fold_subst_s_t in *.
+      repeat rewrite fold_shift_from_t in *.
+      repeat rewrite subst_shift_s_t in *.
+      eauto. 
+    }
+  }
+  {
+    simpl.
+    leO_solver.
+  }
+  {
+    simpl.
+    repeat rewrite fold_subst_s_s in *.
+    repeat rewrite fold_shift_from_s in *.
+    repeat rewrite subst_shift_s_s in *.
+    reflexivity.
+  }
+Qed.
+
+Lemma TPtabs0 T e t :
+  typing (add_kinding 0 T) e t F0 Stt ->
+  typing T (Etabs e) (Tuniversal F0 Stt t) F0 Stt.
+Proof.
+  intros; eapply TPtabs with (n := F0) (s := Stt); simpl; eauto.
+Qed.
+
+Lemma TPsubn T e t n s n' :
+  typing T e t n s ->
+  n <<= n' ->
+  typing T e t n' s.
+Proof.
+  intros; eapply TPsub; eauto.
+  reflexivity.
+Qed.
+
+Lemma TPinl_app T A B e n s :
+  typing T e A n s ->
+  typing T (Einl $$ A $$ B $$ e) (Tsum $$ A $$ B) (n + F1) (Sinl s).
+Proof.
+  intros H.
+  eapply TPsub.
+  {
+    eapply TPapp'.
+    {
+      eapply TPtapp0.
+      {
+        eapply TPtapp0.
+        { eapply TPinl. }
+        { simpl; eauto. }
+      }              
+      { simpl; eauto. }
+    }
+    { 
+      simpl.
+      repeat rewrite fold_shift_from_t in *.
+      repeat rewrite fold_subst_t_t in *.
+      repeat rewrite subst_shift_t_t in *.
+      eauto.
+    }
+    { 
+      simpl.
+      repeat rewrite fold_shift_from_t in *.
+      repeat rewrite fold_subst_s_t in *.
+      repeat rewrite subst_shift_s_t in *.
+      fold (iter 2 (shift_from_t 0) A).
+      repeat rewrite subst_shift_t_t_n in *.
+      simpl.
+      repeat rewrite fold_shift_from_t in *.
+      repeat rewrite fold_subst_s_t in *.
+      repeat rewrite subst_shift_s_t in *.
+      eauto.
+    }
+  }
+  {
+    simpl.
+    leO_solver.
+  }
+  {
+    simpl.
+    reflexivity.
+  }
+Qed.
+
+Lemma TPinr_app T A B e n s :
+  typing T e B n s ->
+  typing T (Einr $$ A $$ B $$ e) (Tsum $$ A $$ B) (n + F1) (Sinr s).
+Proof.
+  intros H.
+  eapply TPsub.
+  {
+    eapply TPapp'.
+    {
+      eapply TPtapp0.
+      {
+        eapply TPtapp0.
+        { eapply TPinr. }
+        { simpl; eauto. }
+      }              
+      { simpl; eauto. }
+    }
+    { eauto. }          
+    { 
+      simpl.
+      repeat rewrite fold_shift_from_t in *.
+      repeat rewrite fold_subst_s_t in *.
+      repeat rewrite subst_shift_s_t in *.
+      fold (iter 2 (shift_from_t 0) A).
+      repeat rewrite subst_shift_t_t_n in *.
+      simpl.
+      repeat rewrite fold_shift_from_t in *.
+      repeat rewrite fold_subst_s_t in *.
+      repeat rewrite subst_shift_s_t in *.
+      eauto.
+    }
+  }
+  {
+    simpl.
+    leO_solver.
+  }
+  {
+    simpl.
+    reflexivity.
+  }
+Qed.
+
+Lemma TPsubs T e t n s s' :
+  typing T e t n s ->
+  s <= s' ->
+  typing T e t n s'.
+Proof.
+  intros; eapply TPsub; eauto.
+  reflexivity.
+Qed.
+
+Lemma is_pair_shift sp s1 s2 : is_pair sp = Some (s1, s2) -> is_pair (shift sp) = Some (shift s1, shift s2).
+Proof.
+  destruct sp; simpl; try discriminate; intros H; inject H; eauto.
+  destruct x.
+  eauto.
+Qed.
+
+Lemma is_hide_shift s s' : is_hide s = Some s' -> is_hide (shift s) = Some (shift s').
+Proof.
+  destruct s; simpl; try discriminate; intros H; inject H; eauto.
+  destruct x.
+  eauto.
+Qed.
+
+Definition shift_from_TE n te :=
+  match te with
+    | TEtyping ty => TEtyping $ shift_from n ty
+    | TEkinding k => te
+  end.
+
+Instance Shift_tc_entry : Shift tc_entry :=
+  {
+    shift_from := shift_from_TE
+  }.
+
+Lemma Kshift a T t k : kinding T t k -> kinding (a :: T) (shift t) k.
+  admit.
+Qed.
+
+Lemma fold_shift_from_e n x : visit_e n (shift_e_f, shift_from) x = shift_from_e n x.
+Proof.
+  eauto.
+Qed.
+
+Definition uncurry {U V W : Type} (f : U -> V -> W) (p : U*V) : W :=
+  f (fst p) (snd p).
+Arguments uncurry {U V W} f p / .
+
+Fixpoint rev_range len :=
+  match len with
+    | 0 => nil
+    | S n => n :: rev_range n
+  end.
+
+Open Scope F.
+
+Lemma subst_shift_from_s_t x : forall v n m, (m <= n)%nat -> subst_size_type m (shift_from_s n v) (shift_from_t (S n) x) = shift_from_t n (subst_size_type m v x).
+  admit.
+Qed.
+Lemma subst_shift_from_s_s x : forall v n m, (m <= n)%nat -> subst_size_size m (shift_from_s n v) (shift_from_s (S n) x) = shift_from_s n (subst_size_size m v x).
+  admit.
+Qed.
+Lemma subst_shift_from_t_t x : forall v n m, (m <= n)%nat -> subst_t_t m (shift_from_t n v) (shift_from_t (S n) x) = shift_from_t n (subst_t_t m v x).
+  admit.
+Qed.
+Lemma shift_from_shift_from_f x n : shift_from_f (S n) (shift_from_f 0 x) = shift_from_f 0 (shift_from_f n x).
+  admit.
+Qed.
+Lemma shift_from_shift_from_s x n : shift_from_s (S n) (shift_from_s 0 x) = shift_from_s 0 (shift_from_s n x).
+  admit.
+Qed.
+Lemma Kinsert T t k : 
+  kinding T t k ->
+  forall T1 skipped T2 T' m,
+    T = T1 ++ T2 ->
+    m = length T1 ->
+    T' = map (uncurry shift_from) (combine (rev_range m) T1) ++ skipped :: T2 ->
+    kinding T' (shift_from m t) k.
+  admit.
+Qed.
+
+Lemma TPlet' T t1 e1 e2 t2 n1 n2 s1 s2 t2' :
+  typing T e1 t1 n1 s1 ->
+  typing (add_typing (t1, Some s1) T) e2 t2 n2 s2 ->
+  t2' = subst s1 t2 ->
+  typing T (Elet t1 e1 e2) t2' (n1 + subst s1 n2) (subst s1 s2).
+Proof.
+  intros; subst; eapply TPlet; eauto.
+Qed.
+
+Lemma TPinsert T e t c s : 
+  typing T e t c s ->
+  forall T1 skipped T2 T' m,
+    T = T1 ++ T2 ->
+    m = length T1 ->
+    T' = map (uncurry shift_from) (combine (rev_range m) T1) ++ skipped :: T2 ->
+    typing T' (shift_from m e) (shift_from m t) (shift_from m c) (shift_from m s).
+Proof.
+  induction 1.
+  {
+    unfold_all; intros T1 skipped T2 T' m ? ? ?; subst.
+    rename n into x.
+    Arguments shift_e_f nv nq / .
+    simpl in *.
+    repeat rewrite fold_shift_from_t in *.
+    repeat rewrite fold_shift_from_s in *.
+    destruct (nat_cmp x (length T1)) as [x' ? Hc | ? | x' ? Hc]; subst.
+    {
+      eapply TPvar'.
+      { simpl.
+        rewrite Bedrock.Expr.nth_error_app_L in H by eauto.
+        eapply Structured.nth_error_app1.
+        etransitivity.
+        {
+          eapply map_nth_error.
+          eapply nth_error_combine.
+          {
+            Lemma nth_error_rev_range len i : i < len -> nth_error (rev_range len) i = Some (len - (1 + i)).
+              admit.
+            Qed.
+            rewrite nth_error_rev_range by eauto.
+            eauto.
+          }
+          { eauto. }
+        }
+        { simpl; eauto. }
+      }
+      { simpl.
+        admit.
+      }
+      admit.
+    }
+    admit.
+    admit.
+  }
+  {
+    unfold_all; intros T1 skipped T2 T' m ? ? ?; subst.
+    simpl in *.
+    repeat rewrite fold_shift_from_s in *.
+    repeat rewrite fold_subst_s_f in *.
+    repeat rewrite fold_shift_from_f in *.
+    repeat rewrite <- subst_shift_from_s_f by omega.
+    repeat rewrite fold_subst_s_s in *.
+    repeat rewrite <- subst_shift_from_s_s by omega.
+    eapply TPapp'.
+    { eapply IHtyping1; eauto. }
+    { eapply IHtyping2; eauto. }
+    simpl.
+    repeat rewrite fold_shift_from_t in *.
+    repeat rewrite fold_subst_s_t in *.
+    repeat rewrite fold_shift_from_s in *.
+    repeat rewrite subst_shift_s_t in *.
+    repeat rewrite subst_shift_from_s_t by omega.
+    eauto.
+  }
+  {
+    unfold_all; intros T1 skipped T2 T' m ? ? ?; subst.
+    simpl in *.
+    eapply TPabs.
+    { eapply Kinsert; eauto. }
+    eapply IHtyping. 
+    { rewrite app_comm_cons.
+      eauto.
+    }
+    { eauto. }
+    { simpl; eauto. }
+  }
+  {
+    unfold_all; intros T1 skipped T2 T' m ? ? ?; subst.
+    simpl in *.
+    eapply TPtapp'.
+    { simpl. 
+      repeat rewrite fold_shift_from_e in *.
+      repeat rewrite fold_shift_from_s in *.
+      repeat rewrite fold_shift_from_f in *.
+      repeat rewrite <- shift_from_shift_from_f in *.
+      repeat rewrite <- shift_from_shift_from_s in *.
+      { eapply IHtyping; eauto. }
+    }
+    simpl.
+    repeat rewrite fold_shift_from_t in *.
+    repeat rewrite fold_subst_t_t in *.
+    repeat rewrite subst_shift_from_t_t by omega.
+    eauto.
+  }
+  {
+    unfold_all; intros T1 skipped T2 T' m ? ? ?; subst.
+    simpl in *.
+    eapply TPtabs.
+    eapply IHtyping. 
+    { rewrite app_comm_cons.
+      eauto.
+    }
+    { eauto. }
+    { simpl; eauto. }
+  }
+  {
+    unfold_all; intros T1 skipped T2 T' m ? ? ?; subst.
+    simpl in *.
+    repeat rewrite fold_shift_from_s in *.
+    repeat rewrite fold_subst_s_f in *.
+    repeat rewrite fold_shift_from_f in *.
+    repeat rewrite <- subst_shift_from_s_f by omega.
+    repeat rewrite fold_subst_s_s in *.
+    repeat rewrite <- subst_shift_from_s_s by omega.
+    eapply TPlet'.
+    { eapply IHtyping1; eauto. }
+    { eapply IHtyping2.
+      { rewrite app_comm_cons.
+        eauto.
+      }
+      { eauto. }
+      { simpl; eauto. }
+    }
+    simpl.
+    repeat rewrite fold_shift_from_t in *.
+    repeat rewrite fold_subst_s_t in *.
+    repeat rewrite fold_shift_from_s in *.
+    repeat rewrite subst_shift_s_t in *.
+    repeat rewrite subst_shift_from_s_t by omega.
+    eauto.
+  }
+  {
+(*
+    unfold_all; intros T1 skipped T2 T' m ? ? ?; subst.
+    simpl.
+    eapply TPletrec.
+    {
+      intros lhs_t rhs_t e Hin.
+      Lemma in_loop A B ls b f : In b ((fix loop (ls : list A) : list B := match ls with [] => [] | x :: xs => f x :: loop xs end) ls) -> exists a, In a ls /\ f a = b.
+        admit.
+      Qed.
+      (*here*)
+      eapply (@in_loop (type * type * expr) (type * type * expr)) in Hin.
+    }
+    repeat rewrite fold_shift_from_s in *.
+    repeat rewrite fold_subst_s_f in *.
+    repeat rewrite fold_shift_from_f in *.
+    repeat rewrite <- subst_shift_from_s_f by omega.
+    repeat rewrite fold_subst_s_s in *.
+    repeat rewrite <- subst_shift_from_s_s by omega.
+    eapply TPlet'.
+    { eapply IHtyping1; eauto. }
+    { eapply IHtyping2.
+      { rewrite app_comm_cons.
+        eauto.
+      }
+      { eauto. }
+      { simpl; eauto. }
+    }
+    simpl.
+    repeat rewrite fold_shift_from_t in *.
+    repeat rewrite fold_subst_s_t in *.
+    repeat rewrite fold_shift_from_s in *.
+    repeat rewrite subst_shift_s_t in *.
+    repeat rewrite subst_shift_from_s_t by omega.
+    eauto.
+*)
+    admit.
+  }
+
+  admit.
+  admit.
+  admit.
+  admit.
+  admit.
+  admit.
+  admit.
+  admit.
+  admit.
+  admit.
+  admit.
+  admit.
+  admit.
+  admit.
+Qed.
+
+Lemma TPinsert2 T e t n s r0 r1 r2 r0' r1' : 
+  typing (r0 :: r1 :: T) e t n s ->
+  r0' = shift_from 1 r0 ->
+  r1' = shift_from 0 r1 ->
+  typing (r0' :: r1' :: r2 :: T) (shift_from 2 e) (shift_from 2 t) (shift_from 2 n) (shift_from 2 s).
+Proof.
+  intros H ? ?; subst.
+  eapply TPinsert; eauto.
+  {
+    instantiate (1 := T).
+    instantiate (1 := [r0; r1]).
+    eauto.
+  }
+  { eauto. }
+  simpl; eauto.
+Qed.
+
+Lemma TPinsert0 T e t n s r : typing T e t n s -> typing (r :: T) (shift e) (shift t) (shift n) (shift s).
+Proof.
+  intros H.
+  eapply TPinsert; eauto.
+  {
+    instantiate (1 := T).
+    instantiate (1 := []).
+    eauto.
+  }
+  { eauto. }
+  simpl; eauto.
+Qed.
+
